Foundation/Modal/Logic/Sublogic/ModalCube.lean
@@ -569,4 +569,10 @@ lemma KD_ssubset_S4 : Logic.KD ⊂ Logic.S4 := by
   . exact KD_ssubset_KT;
   . exact KT_ssubset_S4;
 
+instance : ProperSublogic Logic.Grz Logic.GrzDot2 := ⟨by
+  constructor;
+  . exact Hilbert.weakerThan_of_dominate_axioms (by simp) |>.subset;
+  . sorry;
+⟩
+
 end LO.Modal.Logic
